@prefix dc:      <http://purl.org/dc/elements/1.1/> .
@prefix :        <http://iot.linkeddata.es/def/core#> .
@prefix prov:    <http://www.w3.org/ns/prov#> .
@prefix geo:     <http://www.w3.org/2003/01/geo/wgs84_pos#> .
@prefix foaf:    <http://xmlns.com/foaf/0.1/> .
@prefix ssn:     <http://purl.oclc.org/NET/ssnx/ssn#> .
@prefix vann:    <http://purl.org/vocab/vann/> .
@prefix xml:     <http://www.w3.org/XML/1998/namespace> .
@prefix vs:      <http://www.w3.org/2003/06/sw-vocab-status/ns#> .
@prefix dcterms:  <http://purl.org/dc/terms/> .
@prefix wot:     <http://xmlns.com/wot/0.1/> .
@prefix rdfs:    <http://www.w3.org/2000/01/rdf-schema#> .
@prefix xsd:     <http://www.w3.org/2001/XMLSchema#> .
@prefix owl:     <http://www.w3.org/2002/07/owl#> .
@prefix rdf:     <http://www.w3.org/1999/02/22-rdf-syntax-ns#> .
@prefix saref:   <https://w3id.org/saref#> .
@prefix doap:    <http://usefulinc.com/ns/doap#> .

vs:term_status
      a       owl:AnnotationProperty .

ssn:Selectivity
      a       owl:Class ;
      rdfs:comment "Selectivity is a property of a sensor whereby it provides observed values for one or more qualities such that the values of each quality are independent of other qualities in the phenomenon, body, or substance being investigated." ;
      rdfs:isDefinedBy "http://purl.oclc.org/NET/ssnx/ssn" ;
      rdfs:label "Selectivity" ;
      rdfs:seeAlso "http://www.w3.org/2005/Incubator/ssn/wiki/SSN_Sensor#MeasuringCapability" ;
      rdfs:subClassOf ssn:MeasurementProperty ;
      dc:source """skos:exactMatch 'selectivity' [VIM 4.13]
                                 http://www.bipm.org/utils/common/documents/jcgm/JCGM_200_2008.pdf""" .

:monitors
      a       owl:ObjectProperty ;
      rdfs:isDefinedBy "A link between a sensor an the entities or properties it can monitor."@en ;
      rdfs:label "monitors"@en ;
      rdfs:seeAlso "ISO/IEC CC 30141. Information technology - Internet of Things Reference architecutre (IoT RA)" .

:AmbientProperty
      a       owl:Class ;
      rdfs:label "AmbientProperty"@en ;
      rdfs:subClassOf ssn:Property .

:Thermostat
      a       owl:Class ;
      rdfs:label "Thermostat"@en ;
      rdfs:subClassOf :Actuator , :Sensor .

ssn:Precision
      a       owl:Class ;
      rdfs:comment "The closeness of agreement between replicate observations on an unchanged or similar quality value: i.e., a measure of a sensor's ability to consitently reproduce an observation." ;
      rdfs:isDefinedBy "http://purl.oclc.org/NET/ssnx/ssn" ;
      rdfs:label "Precision" ;
      rdfs:seeAlso "http://www.w3.org/2005/Incubator/ssn/wiki/SSN_Sensor#MeasuringCapability" ;
      rdfs:subClassOf ssn:MeasurementProperty ;
      dc:source """skos:exactMatch 'measurement precision/precision' [VIM 2.15]
                                   http://www.bipm.org/utils/common/documents/jcgm/JCGM_200_2008.pdf""" .

ssn:OperatingRange
      a       owl:Class ;
      rdfs:comment "The environmental conditions and characteristics of a system/sensor's normal operating environment.  Can be used to specify for example the standard environmental conditions in which the sensor is expected to operate (a Condition with no OperatingProperty), or how the environmental and other operating properties relate: i.e., that the maintenance schedule or power requirements differ according to the conditions." ;
      rdfs:isDefinedBy "http://purl.oclc.org/NET/ssnx/ssn" ;
      rdfs:label "Operating Range" ;
      rdfs:seeAlso "http://www.w3.org/2005/Incubator/ssn/wiki/SSN_Deploy#OperatingRestriction" ;
      rdfs:subClassOf ssn:Property ;
      rdfs:subClassOf
              [ a       owl:Restriction ;
                owl:allValuesFrom ssn:OperatingProperty ;
                owl:onProperty ssn:hasOperatingProperty
              ] ;
      rdfs:subClassOf
              [ a       owl:Restriction ;
                owl:allValuesFrom ssn:Condition ;
                owl:onProperty ssn:inCondition
              ] ;
      dc:source """skos:broaderMatch 'reference operating condition' [VIM 4.11]
                                  http://www.bipm.org/utils/common/documents/jcgm/JCGM_200_2008.pdf

The difference is that here we also allow for qualities that aren't VIM influence quantities [VIM 2.52] - for example, a quantity that alters the power requirements, but doesn't affect the measurement properties - conditions specified in MeasurementCapability should be influence quantities.""" .

ssn:hasValue
      a       owl:ObjectProperty ;
      rdfs:isDefinedBy "http://purl.oclc.org/NET/ssnx/ssn"@en ;
      rdfs:label "has value"@en .

ssn:MeasurementProperty
      a       owl:Class ;
      rdfs:comment "An identifiable and observable characteristic of a sensor's observations or ability to make observations." ;
      rdfs:isDefinedBy "http://purl.oclc.org/NET/ssnx/ssn" ;
      rdfs:label "Measurement  Property" ;
      rdfs:seeAlso "http://www.w3.org/2005/Incubator/ssn/wiki/SSN_Sensor#MeasuringCapability" ;
      rdfs:subClassOf ssn:Property .

ssn:Resolution
      a       owl:Class ;
      rdfs:comment "The smallest difference in the value of a quality being observed that would result in perceptably different values of observation results." ;
      rdfs:isDefinedBy "http://purl.oclc.org/NET/ssnx/ssn" ;
      rdfs:label "Resolution" ;
      rdfs:seeAlso "http://www.w3.org/2005/Incubator/ssn/wiki/SSN_Sensor#MeasuringCapability" ;
      rdfs:subClassOf ssn:MeasurementProperty ;
      dc:source """skos:exactMatch 'resolution' [VIM 4.14]
                                  http://www.bipm.org/utils/common/documents/jcgm/JCGM_200_2008.pdf""" .

:AverageMovementTime
      a       owl:NamedIndividual , :MotionProperty ;
      rdfs:label "AverageMovementTime"@en .

:Device
      a       owl:Class ;
      rdfs:comment "An IoT device is a digital entity which bridges between real-world physical entities and the other digital entities of an IoT system. IoT device interacts one or more networks through which interactions are made with other entities. IoT device exposes one or more endpoints by which interactions are made. (definition taken from ISO/IEC 11404:2007)"@en ;
      rdfs:label "Device"@en ;
      rdfs:seeAlso "ISO/IEC CC 30141. Information technology - Internet of Things Reference architecutre (IoT RA)"@en ;
      rdfs:subClassOf :PhysicalThing .

ssn:forProperty
      a       owl:ObjectProperty .

<http://iot.linkeddata.es/def/wot#Event>
      rdfs:subClassOf
              [ a       owl:Restriction ;
                owl:onProperty :monitors ;
                owl:someValuesFrom <http://iot.linkeddata.es/def/wot#Property>
              ] .

:HighestHumidityDeviation
      a       :HumidityAmbientProperty , owl:NamedIndividual ;
      rdfs:label "Highst humidity deviation"@en .

:CO2Sensor
      a       owl:Class ;
      rdfs:label "CO2 Sensor"@en ;
      rdfs:subClassOf :Sensor ;
      rdfs:subClassOf
              [ a       owl:Restriction ;
                owl:onProperty :monitors ;
                owl:someValuesFrom :CarbonDioxide
              ] .

ssn:Frequency
      a       owl:Class ;
      rdfs:comment "The smallest possible time between one observation and the next." ;
      rdfs:isDefinedBy "http://purl.oclc.org/NET/ssnx/ssn" ;
      rdfs:label "Frequency" ;
      rdfs:seeAlso "http://www.w3.org/2005/Incubator/ssn/wiki/SSN_Sensor#MeasuringCapability" ;
      rdfs:subClassOf ssn:MeasurementProperty .

:AverageSoundDeviation
      a       owl:NamedIndividual , :Sound ;
      rdfs:label "Average sound deviation"@en .

:hasValue
      a       owl:ObjectProperty ;
      rdfs:comment "Indicates a value provided by an interaction pattern. In case one ore more values are indicated the order will be defined by the time stamp attributes."@en ;
      rdfs:domain <http://iot.linkeddata.es/def/wot#InteractionPattern> ;
      rdfs:label "has value"@en ;
      rdfs:range :Value .

:Thermometer
      a       owl:Class ;
      rdfs:label "Thermometer"@en ;
      rdfs:subClassOf :Sensor ;
      rdfs:subClassOf
              [ a       owl:Restriction ;
                owl:onProperty :monitors ;
                owl:someValuesFrom :TemperatureAmbientProperty
              ] .

:Mode
      a       :OperationalStatus , owl:NamedIndividual ;
      rdfs:label "Mode"@en .

ssn:inCondition
      a       owl:ObjectProperty .

:MotionSensor
      a       owl:Class ;
      rdfs:label "Motion sensor"@en ;
      rdfs:subClassOf :Sensor ;
      rdfs:subClassOf
              [ a       owl:Restriction ;
                owl:onProperty :monitors ;
                owl:someValuesFrom :MotionProperty
              ] .

:IndoorClimateQualitySensor
      a       owl:Class ;
      rdfs:label "IndoorClimateQualitySensor"@en ;
      rdfs:subClassOf :Sensor .

:Sound
      a       owl:Class ;
      rdfs:label "Sound"@en ;
      rdfs:subClassOf ssn:Property .

:ThingDescription
      a       owl:Class ;
      rdfs:comment "A digital representation encapsulates a physical object accessible via Web services"@en ;
      rdfs:label "Thing description"@en ;
      rdfs:subClassOf
              [ a       owl:Restriction ;
                owl:allValuesFrom <http://iot.linkeddata.es/def/wot#Thing> ;
                owl:onProperty :describes
              ] ;
      rdfs:subClassOf
              [ a       owl:Restriction ;
                owl:onProperty :describes ;
                owl:someValuesFrom <http://iot.linkeddata.es/def/wot#Thing>
              ] .

:AverageMovemenetShare
      a       owl:NamedIndividual , :MotionProperty ;
      rdfs:label "AverageMovemenetShare"@en .

:NoiseLevel
      a       owl:NamedIndividual , :Sound ;
      rdfs:label "Sound level"@en , "Noise level"@en .

:interactsUsing
      a       owl:ObjectProperty ;
      rdfs:isDefinedBy "Linkg between an agent and the virtual thing it interatcs with."@en ;
      rdfs:label "interacts using"@en ;
      rdfs:seeAlso "ISO/IEC CC 30141. Information technology - Internet of Things Reference architecutre (IoT RA)" .

:LuminanceMeter
      a       owl:Class ;
      rdfs:label "Luminance meter"@en ;
      rdfs:subClassOf :Sensor .

:isDescribedBy
      a       owl:ObjectProperty ;
      rdfs:comment "Relation from a thing to its thing descriptions"@en ;
      rdfs:label "is described by"@en .

:describesEcosystem
      a       owl:FunctionalProperty , owl:ObjectProperty ;
      rdfs:comment "Link between a thing ecosystem description and the ecosystem being described."@en ;
      rdfs:label "describes ecosystem"@en ;
      owl:deprecated "true"^^xsd:boolean ;
      owl:inverseOf :isEcosystemDescribedBy .

:HumiditySensor
      a       owl:Class ;
      rdfs:label "Humidity sensor"@en ;
      rdfs:subClassOf :Sensor ;
      rdfs:subClassOf
              [ a       owl:Restriction ;
                owl:onProperty :monitors ;
                owl:someValuesFrom :HumidityAmbientProperty
              ] .

<http://www.loa-cnr.it/ontologies/DUL.owl#hasQuality>
      a       owl:ObjectProperty .

ssn:hasMeasurementProperty
      a       owl:ObjectProperty ;
      rdfs:comment "Relation from a MeasurementCapability to a MeasurementProperty.  For example, to an accuracy (see notes at MeasurementCapability)." ;
      rdfs:isDefinedBy "http://purl.oclc.org/NET/ssnx/ssn" ;
      rdfs:label "has measurement property" ;
      rdfs:seeAlso "http://www.w3.org/2005/Incubator/ssn/wiki/SSN_Sensor#MeasuringCapability" ;
      rdfs:subPropertyOf ssn:hasProperty .

:HumanUser
      a       owl:Class ;
      rdfs:comment "A human user is person who uses an IoT system. A human user is a specialization of an IoT-User. A human user interacts across the network via an application. (definition taken from ISO/IEC 11404:2007)"@en ;
      rdfs:label "Human user"@en ;
      rdfs:seeAlso "ISO/IEC CC 30141. Information technology - Internet of Things Reference architecutre (IoT RA)"@en ;
      rdfs:subClassOf foaf:Person ;
      rdfs:subClassOf
              [ a       owl:Restriction ;
                owl:allValuesFrom :Application ;
                owl:onProperty :interactsUsing
              ] .

ssn:SurvivalProperty
      a       owl:Class ;
      rdfs:comment "An identifiable characteristic that represents the extent of the sensors useful life.  Might include for example total battery life or number of recharges, or, for sensors that are used only a fixed number of times, the number of observations that can be made before the sensing capability is depleted." ;
      rdfs:isDefinedBy "http://purl.oclc.org/NET/ssnx/ssn" ;
      rdfs:label "Survival Property" ;
      rdfs:seeAlso "http://www.w3.org/2005/Incubator/ssn/wiki/SSN_Deploy#OperatingRestriction" ;
      rdfs:subClassOf ssn:Property .

geo:location
      a       owl:ObjectProperty .

:CarbonMonoxide
      a       owl:Class ;
      rdfs:label "CarbonMonoxide"@en ;
      rdfs:subClassOf ssn:Property .

:AverageHumidity
      a       :HumidityAmbientProperty , owl:NamedIndividual ;
      rdfs:label "Average Humidity"@en .

ssn:MaintenanceSchedule
      a       owl:Class ;
      rdfs:comment "Schedule of maintenance for a system/sensor in the specified conditions." ;
      rdfs:isDefinedBy "http://purl.oclc.org/NET/ssnx/ssn" ;
      rdfs:label "Maintenance Schedule" ;
      rdfs:seeAlso "http://www.w3.org/2005/Incubator/ssn/wiki/SSN_Deploy#OperatingRestriction" ;
      rdfs:subClassOf ssn:OperatingProperty .

saref:Service
      a       owl:Class ;
      rdfs:comment "A service is a representation of a function to a network that makes the function discoverable, registerable, remotely controllable by other devices in the network. A service can represent one or more functions. A Service is offered by a device that wants (a certain set of) its function(s) to be discoverable, registerable, remotely controllable by other devices in the network. A Service must specify the device that is offering the service, the function(s) to be represented, and the (input and output) parameters necessary to operate the service."@en ;
      rdfs:isDefinedBy saref: ;
      rdfs:label "Service"@en ;
      vs:term_status "unstable" .

:LightSwitch
      a       owl:Class ;
      rdfs:label "Light switch"@en ;
      rdfs:subClassOf :Actuator .

<http://www.loa-cnr.it/ontologies/DUL.owl#Quality>
      a       owl:Class .

:PhysicalThing
      a       owl:Class ;
      rdfs:comment """A physical entity is a real-world thing. A physical entity is a specialization of entity. A physical entity may contain other physical entities. A physical entity is a discrete, identifiable part of the physical environment that is of interest to the user for the completion of her goal. Physical entities can be almost any physical object or environment; from humans or animals to cars; from store or logistics chain items to computers; from electronic appliances to closed or open environments.

(Definition taken from 
ISO/IEC CC 30141. Information technology - Internet of Things Reference architecutre (IoT RA))"""@en , "Any entity that has a proper space region."@en ;
      rdfs:label "Physical thing"@en ;
      rdfs:seeAlso "ISO/IEC CC 30141. Information technology - Internet of Things Reference architecutre (IoT RA)"@en ;
      rdfs:subClassOf <http://iot.linkeddata.es/def/wot#Thing> , geo:SpatialThing ;
      rdfs:subClassOf
              [ a       owl:Restriction ;
                owl:allValuesFrom :PhysicalThing ;
                owl:onProperty :contains
              ] ;
      rdfs:subClassOf
              [ a       owl:Restriction ;
                owl:allValuesFrom geo:SpatialThing ;
                owl:onProperty geo:location
              ] .

:Presence
      a       owl:Class ;
      rdfs:label "Presence"@en ;
      rdfs:subClassOf ssn:Property .

:Neighbourhood
      a       owl:Class ;
      rdfs:comment "A set of IoT infrastructures and value-added services integrated through a network of VICINITY Nodes, where the infrastructures can share the access to their IoT objects without losing the control over them."@en ;
      rdfs:label "Neighbourhood"@en .

rdfs:Resource
      a       owl:Class .

[]    owl:cardinality "1"^^xsd:nonNegativeInteger .

ssn:DetectionLimit
      a       owl:Class ;
      rdfs:comment "An observed value for which the probability of falsely claiming the absence of a component in a material is Î², given a probability Î± of falsely claiming its presence." ;
      rdfs:isDefinedBy "http://purl.oclc.org/NET/ssnx/ssn" ;
      rdfs:label "detection limit" ;
      rdfs:seeAlso "http://www.w3.org/2005/Incubator/ssn/wiki/SSN_Sensor#MeasuringCapability" ;
      rdfs:subClassOf ssn:MeasurementProperty ;
      dc:source """skos:exactMatch 'detection limit' [VIM 4.18] 
                                 http://www.bipm.org/utils/common/documents/jcgm/JCGM_200_2008.pdf""" .

:MaxLightIntensity
      a       owl:NamedIndividual , :LuminusIntensity ;
      rdfs:label "MaxLightIntensity"@en .

ssn:Accuracy
      a       owl:Class ;
      rdfs:comment "The closeness of agreement between the value of an observation and the true value of the observed quality." ;
      rdfs:isDefinedBy "http://purl.oclc.org/NET/ssnx/ssn" ;
      rdfs:label "Accuracy" ;
      rdfs:seeAlso "http://www.w3.org/2005/Incubator/ssn/wiki/SSN_Sensor#MeasuringCapability" ;
      rdfs:subClassOf ssn:MeasurementProperty ;
      dc:source """skos:exactMatch 'measurement accuracy/accuracy' [VIM 2.13] 
		                    http://www.bipm.org/utils/common/documents/jcgm/JCGM_200_2008.pdf""" .

:MotionProperty
      a       owl:Class ;
      rdfs:label "Motion property"@en ;
      rdfs:subClassOf ssn:Property .

:Lightbulb
      a       owl:Class ;
      rdfs:label "Lightbulb"@en ;
      rdfs:subClassOf :Device .

:serialNumber
      a       owl:DatatypeProperty ;
      rdfs:comment "Device serial number" ;
      rdfs:domain :Device ;
      rdfs:label "serialNumber"@en ;
      rdfs:range xsd:string .

:MinSound
      a       owl:NamedIndividual , :Sound ;
      rdfs:label "MinSound"@en .

ssn:Sensitivity
      a       owl:Class ;
      rdfs:comment "Sensitivity is the quotient of the change in a result of sensor and the corresponding change in a value of a quality being observed." ;
      rdfs:isDefinedBy "http://purl.oclc.org/NET/ssnx/ssn" ;
      rdfs:label "Sensitivity" ;
      rdfs:seeAlso "http://www.w3.org/2005/Incubator/ssn/wiki/SSN_Sensor#MeasuringCapability" ;
      rdfs:subClassOf ssn:MeasurementProperty ;
      dc:source """skos:exactMatch 'sensitivity' [VIM 4.12]
                                  http://www.bipm.org/utils/common/documents/jcgm/JCGM_200_2008.pdf""" .

:Charger
      a       owl:Class ;
      rdfs:label "Charger"@en ;
      rdfs:subClassOf :Device .

:AverageTemperature
      a       owl:NamedIndividual , :TemperatureAmbientProperty ;
      rdfs:label "AverageTemperature"@en .

:hasNeighbourhood
      a       owl:FunctionalProperty , owl:ObjectProperty ;
      rdfs:domain :Agent ;
      rdfs:isDefinedBy "The link between an agent and its neighbourhood. Such neighbourhood will link to all the entities involved in such neighbourhood."@en ;
      rdfs:label "has neighbourhood"@en ;
      rdfs:range :Neighbourhood ;
      rdfs:subPropertyOf :isInvolvedIn ;
      owl:inverseOf :isNeighbourhoodOf .

ssn:SystemLifetime
      a       owl:Class ;
      rdfs:comment "Total useful life of a sensor/system (expressed as total life since manufacture, time in use, number of operations, etc.)." ;
      rdfs:isDefinedBy "http://purl.oclc.org/NET/ssnx/ssn" ;
      rdfs:label "System Lifetime" ;
      rdfs:seeAlso "http://www.w3.org/2005/Incubator/ssn/wiki/SSN_Deploy#OperatingRestriction" ;
      rdfs:subClassOf ssn:SurvivalProperty .

:literalValue
      a       owl:ObjectProperty ;
      rdfs:comment "Literal representation of the observed value."@en ;
      rdfs:domain :Value ;
      rdfs:label "literal value"@en ;
      rdfs:range rdfs:Resource .

:Ecosystem
      a       owl:Class ;
      rdfs:comment "Collection of things that co-exist in a given environment."@en ;
      rdfs:label "Ecosystem"@en ;
      rdfs:subClassOf
              [ a       owl:Restriction ;
                owl:onProperty :isDescribedBy ;
                owl:someValuesFrom :ThingEcosystemDescription
              ] .

<http://www.w3.org/ns/org#Head>
      a       :OperationalStatus .

:serviceDescription
      a       owl:DatatypeProperty ;
      rdfs:comment "Natural language description of a service."@en ;
      rdfs:domain :Service ;
      rdfs:label "service description"@en ;
      rdfs:range xsd:string ;
      rdfs:subPropertyOf :desctiption .

:MaxCO2Concentration
      a       owl:NamedIndividual , :CarbonDioxide ;
      rdfs:label "MaxCO2"@en .

:hasComponent
      a       owl:ObjectProperty ;
      rdfs:comment "A link between an ecosystem and the things that compose such ecosystem."@en ;
      rdfs:label "has component"@en ;
      owl:inverseOf :isComponentOf .

:FanSpeed
      a       :OperationalStatus , owl:NamedIndividual ;
      rdfs:label "FanSpeed"@en .

:WindowSensor
      a       owl:Class ;
      rdfs:label "WindowSensor"@en ;
      rdfs:subClassOf :Sensor ;
      vs:term_status "unstable" .

:CO2Concentration
      a       owl:NamedIndividual , :CarbonDioxide ;
      rdfs:label "CO2Concentration"@en .

:relativeHref
      a       owl:DatatypeProperty ;
      rdfs:domain :RelativeEndpoint ;
      rdfs:label "relative href"@en ;
      rdfs:range xsd:string ;
      rdfs:subPropertyOf <http://iot.linkeddata.es/def/wot#href> .

:Radiance
      a       owl:Class ;
      rdfs:label "Radiance"@en ;
      rdfs:subClassOf :LightProperty .

:OnOff
      a       :OperationalStatus , owl:NamedIndividual ;
      rdfs:label "OnOff"@en .

:Agent
      a       owl:Class ;
      rdfs:comment "An agent is a person or piece of software involved in a VICINITY neighbourhood."@en ;
      rdfs:label "Agent"@en ;
      rdfs:subClassOf foaf:Agent .

:isEcosystemDescribedBy
      a       owl:InverseFunctionalProperty , owl:ObjectProperty ;
      rdfs:comment "Link from an ecosystem to the thing ecosystem descriptions that provide information about such ecosystem."@en ;
      rdfs:label "is ecosystem described by"@en ;
      owl:deprecated "true"^^xsd:boolean .

:AverageLightIntensity
      a       owl:NamedIndividual , :LuminusIntensity ;
      rdfs:label "AverageLightIntensity"@en .

:Value
      a       owl:Class ;
      rdfs:comment "Class representing values provided by an interaction pattern in a given time stamp. It might also indicated the data format in which the value is expressed. It can be also be used to express operating property or measurement capability values for a given device."@en ;
      rdfs:label "Value"@en ;
      rdfs:subClassOf
              [ a       owl:Restriction ;
                owl:maxQualifiedCardinality
                        "1"^^xsd:nonNegativeInteger ;
                owl:onDataRange xsd:dateTime ;
                owl:onProperty :timeStamp
              ] ;
      rdfs:subClassOf
              [ a       owl:Restriction ;
                owl:allValuesFrom <http://iot.linkeddata.es/def/wot#DataSchema> ;
                owl:onProperty :expressedInFormat
              ] .

:Motion
      a       owl:NamedIndividual , :MotionProperty ;
      rdfs:label "Motion"@en .

:isInvolvedIn
      a       owl:ObjectProperty ;
      rdfs:isDefinedBy "A link between an agent and all the neighbouthoods it is involved in."@en ;
      rdfs:label "is involved in"@en .

<http://iot.linkeddata.es/def/wot#Action>
      rdfs:subClassOf
              [ a       owl:Restriction ;
                owl:onProperty :actsOn ;
                owl:someValuesFrom ssn:Property
              ] .

ssn:OperatingPowerRange
      a       owl:Class ;
      rdfs:comment "Power range in which system/sensor is expected to operate." ;
      rdfs:isDefinedBy "http://purl.oclc.org/NET/ssnx/ssn" ;
      rdfs:label "Operating Power Range" ;
      rdfs:seeAlso "http://www.w3.org/2005/Incubator/ssn/wiki/SSN_Energy#EnergyRestriction" ;
      rdfs:subClassOf ssn:OperatingProperty .

:PowerMeter
      a       owl:Class ;
      rdfs:label "PowerMeter"@en ;
      rdfs:subClassOf :Sensor .

:Luminance
      a       owl:NamedIndividual , :LuminusIntensity ;
      rdfs:label "Luminance"@en .

:MinLightIntensity
      a       owl:NamedIndividual , :LuminusIntensity ;
      rdfs:label "MinLightIntensity"@en .

:ValvePosition
      a       :OperationalStatus , owl:NamedIndividual ;
      rdfs:label "ValvePosition"@en .

:involves
      a       owl:ObjectProperty ;
      rdfs:isDefinedBy "A link between a neighbourhood and all the agents involved in it."@en ;
      rdfs:label "involves"@en ;
      owl:inverseOf :isInvolvedIn .

:AverageCO2ConcentrationDeviation
      a       owl:NamedIndividual , :CarbonDioxide ;
      rdfs:label "AverageCO2Deviation"@en .

:actsOn
      a       owl:ObjectProperty ;
      rdfs:comment "A link between an actuator an the entities or properties upon which it can act." ;
      rdfs:label "acts on"@en ;
      rdfs:seeAlso "ISO/IEC CC 30141. Information technology - Internet of Things Reference architecutre (IoT RA)" .

:DoorSensor
      a       owl:Class ;
      rdfs:label "DoorSensor"@en ;
      rdfs:subClassOf :Sensor ;
      vs:term_status "unstable" .

:MaxSound
      a       owl:NamedIndividual , :Sound ;
      rdfs:label "MaxSound"@en .

:DimmingLevel
      a       :OperationalStatus , owl:NamedIndividual ;
      rdfs:label "DimmingLevel"@en .

:Actuator
      a       owl:Class ;
      rdfs:comment "An actuator is a device that accepts digital inputs and which acts on (changes) one or more properties of a physical entity on the basis of those inputs. An actuator is a specialization of an IoT device. An actuator acts on a physical entity. (definition taken from ISO/IEC 11404:2007)"@en ;
      rdfs:label "Actuator"@en ;
      rdfs:seeAlso "ISO/IEC CC 30141. Information technology - Internet of Things Reference architecutre (IoT RA)"@en ;
      rdfs:subClassOf :Device ;
      rdfs:subClassOf
              [ a       owl:Restriction ;
                owl:allValuesFrom <http://iot.linkeddata.es/def/wot#Property> ;
                owl:onProperty :actsOn
              ] .

ssn:hasOperatingRange
      a       owl:ObjectProperty ;
      rdfs:comment "Relation from a System to an OperatingRange describing the normal operating environment of the System." ;
      rdfs:isDefinedBy "http://purl.oclc.org/NET/ssnx/ssn" ;
      rdfs:label "has operating range" ;
      rdfs:seeAlso "http://www.w3.org/2005/Incubator/ssn/wiki/SSN_Deploy#OperatingRestriction" ;
      rdfs:subPropertyOf ssn:hasProperty .

:ChargeStatus
      a       :OperationalStatus , owl:NamedIndividual ;
      rdfs:label "ChargeStatus"@en .

ssn:hasOperatingProperty
      a       owl:ObjectProperty ;
      rdfs:comment "Relation from an OperatingRange to a Property.  For example, to a battery lifetime." ;
      rdfs:isDefinedBy "http://purl.oclc.org/NET/ssnx/ssn" ;
      rdfs:label "has operating property" ;
      rdfs:seeAlso "http://www.w3.org/2005/Incubator/ssn/wiki/SSN_Deploy#OperatingRestriction" ;
      rdfs:subPropertyOf ssn:hasProperty .

:HighestSoundDeviation
      a       owl:NamedIndividual , :Sound ;
      rdfs:label "HighestSoundDeviation"@en .

:deviceName
      a       owl:DatatypeProperty ;
      rdfs:comment "Name of a device" ;
      rdfs:domain :Device ;
      rdfs:label "device name"@en ;
      rdfs:range xsd:string ;
      rdfs:subPropertyOf <http://iot.linkeddata.es/def/wot#name> .

ssn:hasProperty
      a       owl:ObjectProperty ;
      rdfs:comment "A relation between a FeatureOfInterest and a Property of that feature." ;
      rdfs:isDefinedBy "http://purl.oclc.org/NET/ssnx/ssn" ;
      rdfs:label "has property" ;
      rdfs:seeAlso "http://www.w3.org/2005/Incubator/ssn/wiki/SSN_Skeleton#Skeleton" ;
      rdfs:subPropertyOf <http://www.loa-cnr.it/ontologies/DUL.owl#hasQuality> ;
      owl:inverseOf ssn:isPropertyOf .

:AverageHumidityDeviation
      a       :HumidityAmbientProperty , owl:NamedIndividual ;
      rdfs:label "Average humidity deviation"@en .

dcterms:contributor
      a       owl:AnnotationProperty .

ssn:Condition
      a       owl:Class ;
      rdfs:comment "Used to specify ranges for qualities that act as conditions on a system/sensor's operation.  For example, wind speed of 10-60m/s is expressed as a condition linking a quality, wind speed, a unit of measurement, metres per second, and a set of values, 10-60, and may be used as the condition on a MeasurementProperty, for example, to state that a sensor has a particular accuracy in that condition." ;
      rdfs:isDefinedBy "http://purl.oclc.org/NET/ssnx/ssn" ;
      rdfs:label "Condition" ;
      rdfs:seeAlso "http://www.w3.org/2005/Incubator/ssn/wiki/SSN_Base#ConstraintBlock" ;
      rdfs:subClassOf ssn:Property .

:VirtualThing
      a       owl:Class ;
      rdfs:comment """A virtual entity is a digital representation of a physical entity, contained within a service. A virtual entity interacts through an endpoint. A virtual entity represents a physical entity.

(Definition taken from 
ISO/IEC CC 30141. Information technology - Internet of Things Reference architecutre (IoT RA))"""@en ;
      rdfs:label "Virtual thing"@en ;
      rdfs:seeAlso "ISO/IEC CC 30141. Information technology - Internet of Things Reference architecutre (ioT RA)"@en ;
      rdfs:subClassOf <http://iot.linkeddata.es/def/wot#Thing> ;
      rdfs:subClassOf
              [ a       owl:Restriction ;
                owl:allValuesFrom :VirtualThing ;
                owl:onProperty :contains
              ] .

ssn:isPropertyOf
      a       owl:ObjectProperty .

owl:cardinality
      a       owl:AnnotationProperty .

:MinHumidity
      a       :HumidityAmbientProperty , owl:NamedIndividual ;
      rdfs:label "Minimun humidity"@en .

:owns
      a       owl:ObjectProperty ;
      rdfs:isDefinedBy "A linkd between an agent and the entities, like devices or services, it provides or owns."@en ;
      rdfs:label "provides"@en , "owns"@en .

:AverageTemperatureDeviation
      a       owl:NamedIndividual , :TemperatureAmbientProperty ;
      rdfs:label "AverageTemperatureDeviation"@en .

:OccupancySensor
      a       owl:Class ;
      rdfs:label "Occupancy sensor"@en ;
      rdfs:subClassOf :Sensor .

foaf:depiction
      a       owl:ObjectProperty .

:HighestTemperatureDeviation
      a       owl:NamedIndividual , :TemperatureAmbientProperty ;
      rdfs:label "Highst temperature deviation"@en .

ssn:hasMeasurementCapability
      a       owl:ObjectProperty ;
      rdfs:comment "Relation from a Sensor to a MeasurementCapability describing the measurement properties of the sensor." ;
      rdfs:isDefinedBy "http://purl.oclc.org/NET/ssnx/ssn" ;
      rdfs:label "has measurement  capability" ;
      rdfs:seeAlso "http://www.w3.org/2005/Incubator/ssn/wiki/SSN_Sensor#MeasuringCapability" ;
      rdfs:subPropertyOf ssn:hasProperty .

:hasOwner
      a       owl:ObjectProperty ;
      rdfs:isDefinedBy "Link between an entity like a service or a device and its owners or providers."@en ;
      rdfs:label "has owner"@en , "has provider"@en ;
      owl:inverseOf :owns .

:MinCO2Concentration
      a       owl:NamedIndividual , :CarbonDioxide ;
      rdfs:label "MinCO2"@en .

:HVACSensor
      a       owl:Class ;
      rdfs:label "HVAC Sensor"@en ;
      rdfs:subClassOf :Actuator , :Sensor .

<https://w3id.org/def/saref4bldg#BuildingSpace>
      a       owl:Class ;
      rdfs:comment "An entity used to define the physical spaces of the building. A building space contains devices or building objects."@en ;
      rdfs:isDefinedBy <https://w3id.org/def/saref4bldg#> ;
      rdfs:label "Building space"@en .

:PowerConsumption
      a       owl:Class ;
      rdfs:label "PowerConsumption"@en ;
      rdfs:subClassOf ssn:OperatingProperty .

:NoiseSensor
      a       owl:Class ;
      rdfs:label "Noise sensor"@en ;
      rdfs:subClassOf :Sensor .

:contains
      a       owl:ObjectProperty ;
      rdfs:comment "A property between a thing and its components. For example, virtual things can contain virtual things while physical things can contain physicial things."@en ;
      rdfs:label "contains"@en ;
      rdfs:seeAlso "ISO/IEC CC 30141. Information technology - Internet of Things Reference architecutre (ioT RA)" .

ssn:FeatureOfInterest
      a       owl:Class ;
      rdfs:isDefinedBy "http://purl.oclc.org/NET/ssnx/ssn" .

:Irradiance
      a       owl:Class ;
      rdfs:label "Irradiance"@en ;
      rdfs:subClassOf :LightProperty .

:hasVendor
      a       owl:ObjectProperty ;
      rdfs:isDefinedBy "Link from a device to its vendor or manufacturer or producer."@en ;
      rdfs:label "has producer"@en , "has vendor"@en .

:isNeighbourhoodOf
      a       owl:FunctionalProperty , owl:ObjectProperty ;
      rdfs:domain :Neighbourhood ;
      rdfs:isDefinedBy "A link between a neighbourhood and the specific agent around which the neighbourhood is built."@en ;
      rdfs:label "is neighbourhood of"@en ;
      rdfs:range :Agent ;
      rdfs:subPropertyOf :involves .

:OperationalStatus
      a       owl:Class ;
      rdfs:label "Operational status"@en ;
      rdfs:subClassOf ssn:Property .

:MinPowerConsumption
      a       :PowerConsumption , owl:NamedIndividual ;
      rdfs:label "MinPowerConsumption"@en .

:hasPartnershipWith
      a       owl:ObjectProperty , owl:SymmetricProperty ;
      rdfs:domain <http://www.w3.org/ns/org#Organization> ;
      rdfs:isDefinedBy "A link between two organizations who are in a partnership relation. A partnership is established between organizations, only 2 organizations."@en ;
      rdfs:label "hasPartnershipWith"@en ;
      rdfs:range <http://www.w3.org/ns/org#Organization> .

dc:source
      a       owl:AnnotationProperty .

:describes
      a       owl:ObjectProperty ;
      rdfs:comment "Link from a thing description to the thing being described"@en ;
      rdfs:label "describes thing"@en ;
      owl:inverseOf :isDescribedBy .

:LightColor
      a       owl:NamedIndividual , :LightProperty ;
      rdfs:label "Light color"@en .

:AmbientTemperature
      a       owl:NamedIndividual , :TemperatureAmbientProperty ;
      rdfs:label "AmbientTemperature"@en .

:RelativeEndpoint
      a       owl:Class ;
      rdfs:comment "An endpoint which is relative (its href is composed by a relative path and an absolute one given by another endpoint) to an endpoint which can not be relative."@en ;
      rdfs:label "Relative endpoint"@en ;
      rdfs:subClassOf <http://iot.linkeddata.es/def/wot#Link> ;
      rdfs:subClassOf
              [ a       owl:Restriction ;
                owl:maxQualifiedCardinality
                        "1"^^xsd:nonNegativeInteger ;
                owl:onClass
                        [ a       owl:Class ;
                          owl:intersectionOf (<http://iot.linkeddata.es/def/wot#Link> [ a       owl:Class ;
                                      owl:complementOf :RelativeEndpoint
                                    ])
                        ] ;
                owl:onProperty :isRelativeTo
              ] .

:EntryExit
      a       owl:NamedIndividual , :Presence ;
      rdfs:label "EntryExit"@en .

:serviceName
      a       owl:DatatypeProperty ;
      rdfs:comment "Name of a service" ;
      rdfs:domain :Service ;
      rdfs:label "service name"@en ;
      rdfs:range xsd:string ;
      rdfs:subPropertyOf <http://iot.linkeddata.es/def/wot#name> .

:EBikeCharger
      a       owl:Class ;
      rdfs:label "eBikeCharger"@en ;
      rdfs:subClassOf :Charger .

ssn:BatteryLifetime
      a       owl:Class ;
      rdfs:comment "Total useful life of a battery." ;
      rdfs:isDefinedBy "http://purl.oclc.org/NET/ssnx/ssn" ;
      rdfs:label "Battery Lifetime" ;
      rdfs:seeAlso "http://www.w3.org/2005/Incubator/ssn/wiki/SSN_Energy#EnergyRestriction" ;
      rdfs:subClassOf ssn:SurvivalProperty .

:MinTemperature
      a       owl:NamedIndividual , :TemperatureAmbientProperty ;
      rdfs:label "Minimun temperature"@en .

<http://iot.linkeddata.es/def/wot#PhysicalThing>
      a       owl:Class .

ssn:Latency
      a       owl:Class ;
      rdfs:comment "The time between a request for an observation and the sensor providing a result." ;
      rdfs:isDefinedBy "http://purl.oclc.org/NET/ssnx/ssn" ;
      rdfs:label "Latency" ;
      rdfs:seeAlso "http://www.w3.org/2005/Incubator/ssn/wiki/SSN_Sensor#MeasuringCapability" ;
      rdfs:subClassOf ssn:MeasurementProperty .

:timeStamp
      a       owl:FunctionalProperty , owl:DatatypeProperty ;
      rdfs:comment "Time stamp in which a phenomenon takes place, for example when value has been taken."@en ;
      rdfs:label "time stamp"@en ;
      rdfs:range xsd:dateTime .

:LuminusIntensity
      a       owl:Class ;
      rdfs:label "LuminusIntensity"@en ;
      rdfs:subClassOf :LightProperty .

:AverageCO2Concentration
      a       owl:NamedIndividual , :CarbonDioxide ;
      rdfs:label "AverageCO2"@en .

:HighestCO2ConcentrationDeviation
      a       owl:NamedIndividual , :CarbonDioxide ;
      rdfs:label "HighestCO2Deviation"@en .

:TemperatureAmbientProperty
      a       owl:Class ;
      rdfs:label "TemperatureAmbientProperty"@en ;
      rdfs:subClassOf :AmbientProperty .

:DigitalUser
      a       owl:Class ;
      rdfs:comment "A digital user is a digital entity which uses an IoT system. A digital user is a specialization of an IoT-User. A digital user interacts with one or more services offered by the IoT system across the network. (definition taken from ISO/IEC 11404:2007)"@en ;
      rdfs:label "Digital user"@en ;
      rdfs:seeAlso "ISO/IEC CC 30141. Information technology - Internet of Things Reference architecutre (IoT RA)"@en ;
      rdfs:subClassOf foaf:Agent ;
      rdfs:subClassOf
              [ a       owl:Restriction ;
                owl:allValuesFrom :Service ;
                owl:onProperty :interactsUsing
              ] .

ssn:ResponseTime
      a       owl:Class ;
      rdfs:comment "The time between a (step) change inthe value of an observed quality and a sensor (possibly with specified error) 'settling' on an observed value." ;
      rdfs:isDefinedBy "http://purl.oclc.org/NET/ssnx/ssn" ;
      rdfs:label "Response time" ;
      rdfs:seeAlso "http://www.w3.org/2005/Incubator/ssn/wiki/SSN_Sensor#MeasuringCapability" ;
      rdfs:subClassOf ssn:MeasurementProperty ;
      dc:source """skos:exactMatch 'step response time' [VIM 4.23]
                                  http://www.bipm.org/utils/common/documents/jcgm/JCGM_200_2008.pdf""" .

:RelativeHumidity
      a       :HumidityAmbientProperty , owl:NamedIndividual ;
      rdfs:label "RelativeHumidity"@en .

ssn:hasSurvivalProperty
      a       owl:ObjectProperty ;
      rdfs:comment "Relation from a SurvivalRange to a Property describing the survial range of a system.  For example, to the temperature extreme that a system can withstand before being considered damaged." ;
      rdfs:isDefinedBy "http://purl.oclc.org/NET/ssnx/ssn" ;
      rdfs:label "has survival property" ;
      rdfs:seeAlso "http://www.w3.org/2005/Incubator/ssn/wiki/SSN_Deploy#OperatingRestriction" ;
      rdfs:subPropertyOf ssn:hasProperty .

:OpenClosed
      a       :OperationalStatus , owl:NamedIndividual ;
      rdfs:label "OpenClosed"@en .

foaf:Image
      a       owl:Class .

<http://iot.linkeddata.es/def/wot#Property>
      rdfs:subClassOf
              [ a       owl:Restriction ;
                owl:onProperty :monitors ;
                owl:someValuesFrom ssn:Property
              ] .

:MaxPowerConsumption
      a       :PowerConsumption , owl:NamedIndividual ;
      rdfs:label "MaxPowerConsumption"@en .

:expressedInFormat
      a       owl:ObjectProperty ;
      rdfs:comment "Link from a value to the data format in which it is expressed."@en ;
      rdfs:domain :Value ;
      rdfs:label "expressed in format"@en ;
      rdfs:range <http://iot.linkeddata.es/def/wot#DataSchema> .

:deviceDescription
      a       owl:DatatypeProperty ;
      rdfs:comment "Natural language description of a device."@en ;
      rdfs:domain :Device ;
      rdfs:label "device description"@en ;
      rdfs:range xsd:string ;
      rdfs:subPropertyOf :desctiption .

:PeopleCounter
      a       owl:Class ;
      rdfs:comment "A people counter is a device that is used to measure the number of people traversing a certain passage or entrance. (Definition taken from https://en.wikipedia.org/wiki/People_counter)"@en ;
      rdfs:label "People counter"@en ;
      rdfs:subClassOf :Sensor ;
      rdfs:subClassOf
              [ a       owl:Restriction ;
                owl:onProperty :monitors ;
                owl:someValuesFrom :Presence
              ] .

:ThingEcosystemDescription
      a       owl:Class ;
      rdfs:comment "A digital representation that encapsulates an ecosystem taht is accessible via Web services" ;
      rdfs:label "Thing ecosystem description"@en ;
      rdfs:subClassOf
              [ a       owl:Restriction ;
                owl:onProperty :describes ;
                owl:someValuesFrom :Ecosystem
              ] .

:MaxHumidity
      a       :HumidityAmbientProperty , owl:NamedIndividual ;
      rdfs:label "MaxHumidity"@en .

:RadiantIntensity
      a       owl:Class ;
      rdfs:label "Radiant intensity"@en ;
      rdfs:subClassOf :LightProperty .

ssn:Property
      a       owl:Class ;
      rdfs:comment "A ssn:Property is something that is a DUL:Quality and has a ssn:isPropertyOf property who may be a ssn:FeatureOfInterest"@en , "An observable Quality of an Event or Object.  That is, not a quality of an abstract entity as is also allowed by DUL's Quality, but rather an aspect of an entity that is intrinsic to and cannot exist without the entity and is observable by a sensor." ;
      rdfs:isDefinedBy "http://purl.oclc.org/NET/ssnx/ssn#" , "http://purl.oclc.org/NET/ssnx/ssn" ;
      rdfs:label "property (ssn)" , "Property" ;
      rdfs:seeAlso "http://www.w3.org/2005/Incubator/ssn/wiki/SSN_Skeleton#Skeleton" ;
      rdfs:subClassOf <http://www.loa-cnr.it/ontologies/DUL.owl#Quality> ;
      rdfs:subClassOf
              [ a       owl:Restriction ;
                owl:onProperty ssn:isPropertyOf ;
                owl:someValuesFrom ssn:FeatureOfInterest
              ] ;
      dc:source """skos:exactMatch 'property' [O&M] 
		                    http://www.opengeospatial.org/standards/om""" .

ssn:MeasurementCapability
      a       owl:Class ;
      rdfs:comment """Collects together measurement properties (accuracy, range, precision, etc) and the environmental conditions in which those properties hold, representing a specification of a sensor's capability in those conditions.

The conditions specified here are those that affect the measurement properties, while those in OperatingRange represent the sensor's standard operating conditions, including conditions that don't affect the observations.""" ;
      rdfs:isDefinedBy "http://purl.oclc.org/NET/ssnx/ssn" ;
      rdfs:label "Measurement Capability" ;
      rdfs:seeAlso "http://www.w3.org/2005/Incubator/ssn/wiki/SSN_Sensor#MeasuringCapability" ;
      rdfs:subClassOf ssn:Property ;
      rdfs:subClassOf
              [ a       owl:Restriction ;
                owl:allValuesFrom ssn:Condition ;
                owl:onProperty ssn:inCondition
              ] ;
      rdfs:subClassOf
              [ a       owl:Restriction ;
                owl:allValuesFrom ssn:MeasurementProperty ;
                owl:onProperty ssn:hasMeasurementProperty
              ] ;
      rdfs:subClassOf
              [ a       owl:Restriction ;
                owl:allValuesFrom ssn:Property ;
                owl:onProperty ssn:forProperty
              ] ;
      dc:source """Similar idea to MeasurementCapability in MMI Device Ontology
                                  http://marinemetadata.org/community/teams/ontdevices

But the the two express the relationship between constraints and multiple measurement properties differently.

The conditions linked to a MeasurementCapability are skos:exactMatch to 'influence quantity' [VIM 2.52]
http://www.bipm.org/utils/common/documents/jcgm/JCGM_200_2008.pdf""" .

:WaterEnergyMeter
      a       owl:Class ;
      rdfs:label "WaterEnergyMeter"@en ;
      rdfs:subClassOf :Sensor .

:Sensor
      a       owl:Class ;
      rdfs:comment "A sensor is a device that detects and responds to some type of input from the physical environment and outputs digital data that can be transmitted over a network. A sensor is a specialization of an IoT device. A sensor monitors a physical entity. The output digital data may only be distantly related to the input from the physical environment and may be output with a significant time delay, depending on processing of the data within the device, for example, the recognition of the identity of a person from a surveillance camera device. (definition taken from ISO/IEC 11404:2007)"@en ;
      rdfs:label "Sensor"@en ;
      rdfs:seeAlso "ISO/IEC CC 30141. Information technology - Internet of Things Reference architecutre (IoT RA)"@en ;
      rdfs:subClassOf :Device ;
      rdfs:subClassOf
              [ a       owl:Restriction ;
                owl:allValuesFrom <http://iot.linkeddata.es/def/wot#Property> ;
                owl:onProperty :monitors
              ] .

:LightProperty
      a       owl:Class ;
      rdfs:label "LightProperty"@en ;
      rdfs:subClassOf ssn:Property .

ssn:SurvivalRange
      a       owl:Class ;
      rdfs:comment "The conditions a sensor can be exposed to without damage: i.e., the sensor continues to operate as defined using MeasurementCapability.  If, however, the SurvivalRange is exceeded, the sensor is 'damaged' and MeasurementCapability specifications may no longer hold." ;
      rdfs:isDefinedBy "http://purl.oclc.org/NET/ssnx/ssn" ;
      rdfs:label "Survival Range" ;
      rdfs:seeAlso "http://www.w3.org/2005/Incubator/ssn/wiki/SSN_Deploy#OperatingRestriction" ;
      rdfs:subClassOf ssn:Property ;
      rdfs:subClassOf
              [ a       owl:Restriction ;
                owl:allValuesFrom ssn:Condition ;
                owl:onProperty ssn:inCondition
              ] ;
      rdfs:subClassOf
              [ a       owl:Restriction ;
                owl:allValuesFrom ssn:SurvivalProperty ;
                owl:onProperty ssn:hasSurvivalProperty
              ] ;
      dc:source """skos:narrowerMatch 'limiting operating condition' [VIM 4.10]
                                  http://www.bipm.org/utils/common/documents/jcgm/JCGM_200_2008.pdf""" .

<https://w3id.org/def/saref4bldg#isContainedIn>
      a       owl:ObjectProperty ;
      rdfs:comment "A relation between an object and the physical space in which it is located."@en ;
      rdfs:isDefinedBy "https://w3id.org/def/saref4bldg#"@en ;
      rdfs:label "is contained in"@en .

ssn:MeasurementRange
      a       owl:Class ;
      rdfs:comment "The set of values that the sensor can return as the result of an observation under the defined conditions with the defined measurement properties.  (If no conditions are specified or the conditions do not specify a range for the observed qualities, the measurement range is to be taken as the condition for the observed qualities.)" ;
      rdfs:isDefinedBy "http://purl.oclc.org/NET/ssnx/ssn" ;
      rdfs:label "Measurement  Range" ;
      rdfs:seeAlso "http://www.w3.org/2005/Incubator/ssn/wiki/SSN_Sensor#MeasuringCapability" ;
      rdfs:subClassOf ssn:MeasurementProperty ;
      dc:source """skos:exactMatch 'measuring interval/measurement range' [VIM 4.7]
                                  http://www.bipm.org/utils/common/documents/jcgm/JCGM_200_2008.pdf""" .

ssn:OperatingProperty
      a       owl:Class ;
      rdfs:comment "An identifiable characteristic of the environmental and other conditions in which the sensor is intended to operate.  May include power ranges, power sources, standard configurations, attachments and the like." ;
      rdfs:isDefinedBy "http://purl.oclc.org/NET/ssnx/ssn" ;
      rdfs:label "Operating Property" ;
      rdfs:seeAlso "http://www.w3.org/2005/Incubator/ssn/wiki/SSN_Deploy#OperatingRestriction" ;
      rdfs:subClassOf ssn:Property .

:WaterFlowMeter
      a       owl:Class ;
      rdfs:label "WaterFlowMeter"@en ;
      rdfs:subClassOf :Sensor .

:IndoorEnvironmentalQualityScore
      a       owl:NamedIndividual , :AmbientProperty ;
      rdfs:label "Indoor environmental quality score"@en , "IEQ score"@en .

:CarbonDioxide
      a       owl:Class ;
      rdfs:label "CarbonDioxide"@en ;
      rdfs:subClassOf ssn:Property .

:AverageSound
      a       owl:NamedIndividual , :Sound ;
      rdfs:label "AverageSound"@en .

ssn:hasSurvivalRange
      a       owl:ObjectProperty ;
      rdfs:comment "A Relation from a System to a SurvivalRange." ;
      rdfs:isDefinedBy "http://purl.oclc.org/NET/ssnx/ssn" ;
      rdfs:label "has survival range" ;
      rdfs:seeAlso "http://www.w3.org/2005/Incubator/ssn/wiki/SSN_Deploy#OperatingRestriction" ;
      rdfs:subPropertyOf ssn:hasProperty .

:desctiption
      a       owl:DatatypeProperty ;
      rdfs:comment "General attribute for descriptions assigned to any type of concept" ;
      rdfs:label "desctiption"@en ;
      rdfs:range xsd:string .

:avatar
      a       owl:ObjectProperty ;
      rdfs:comment "A link from an entity to the image identifying it in a social network or system."@en ;
      rdfs:label "avatar"@en ;
      rdfs:subPropertyOf foaf:depiction .

ssn:qualityOfObservation
      a       owl:ObjectProperty ;
      rdfs:comment "Relation linking an Observation to the adjudged quality of the result.  This is of course complimentary to the MeasurementCapability information recorded for the Sensor that made the Observation." ;
      rdfs:isDefinedBy "http://purl.oclc.org/NET/ssnx/ssn" ;
      rdfs:label "quality of observation" ;
      rdfs:seeAlso "http://www.w3.org/2005/Incubator/ssn/wiki/SSN_Observation#Observation" ;
      rdfs:subPropertyOf ssn:hasProperty ;
      dc:source """skos:exactMatch 'resultQuality' [O&M - ISO/DIS 19156] 
		                    http://portal.opengeospatial.org/files/?artifact_id=41579""" .

:isComponentOf
      a       owl:ObjectProperty ;
      rdfs:comment "A link between a thing and the ecosystems it belongs to."@en ;
      rdfs:label "is component of"@en .

:MeanPowerConsumption
      a       :PowerConsumption , owl:NamedIndividual ;
      rdfs:label "MeanPowerConsumption"@en .

:     a       owl:Ontology ;
      rdfs:comment "This ontology represent the core terms to allow interoperability in an IoT context based on  VICINITY technological solutions."@en ;
      dc:publisher <http://www.oeg-upm.net/> ;
      dc:title "Vicinity core model"@en ;
      dcterms:contributor <http://www.oeg-upm.net/index.php/en/universitystaff/402-fserena/> ;
      dcterms:creator <http://purl.org/net/mpoveda> , <http://www.garcia-castro.com/foaf.rdf#me> ;
      dcterms:license <http://purl.org/NET/rdflicense/cc-by4.0> ;
      vann:preferredNamespacePrefix
              "vcnt-core" ;
      vann:preferredNamespaceUri
              "http://iot.linkeddata.es/def/core" ;
      owl:imports <http://iot.linkeddata.es/def/wot#> , <http://www.w3.org/ns/org#> ;
      owl:versionInfo "0.0.6" .

:isRelativeTo
      a       owl:ObjectProperty ;
      rdfs:comment "Link from a relative endpoint to the (non relative) endpoint to which it is relative."@en ;
      rdfs:label "is relative to"@en .

:Application
      a       owl:Class ;
      rdfs:comment "An application is a software entity or system that offers a collection of functions with which a user can perform a task or achieve a business objective. An application typically uses services. The functions of an application may be presented as services. (definition taken from ISO/IEC 11404:2007)"@en ;
      rdfs:label "Application"@en ;
      rdfs:seeAlso "ISO/IEC CC 30141. Information technology - Internet of Things Reference architecutre (IoT RA)"@en ;
      rdfs:subClassOf :Service .

ssn:Drift
      a       owl:Class ;
      rdfs:comment "A, continuous or incremental, change in the reported values of observations over time for an unchanging quality." ;
      rdfs:isDefinedBy "http://purl.oclc.org/NET/ssnx/ssn" ;
      rdfs:label "Drift" ;
      rdfs:seeAlso "http://www.w3.org/2005/Incubator/ssn/wiki/SSN_Sensor#MeasuringCapability" ;
      rdfs:subClassOf ssn:MeasurementProperty ;
      dc:source """skos:exactMatch 'instrumental drift' [VIM 4.21]
                                  http://www.bipm.org/utils/common/documents/jcgm/JCGM_200_2008.pdf""" .

geo:SpatialThing
      a       owl:Class .

:MaxTemperature
      a       owl:NamedIndividual , :TemperatureAmbientProperty ;
      rdfs:label "MaxTemperature"@en .

:LuminusFlux
      a       owl:Class ;
      rdfs:label "Luminus flux"@en ;
      rdfs:subClassOf :LightProperty .

:HumidityAmbientProperty
      a       owl:Class ;
      rdfs:label "HumidityAmbientProperty"@en ;
      rdfs:subClassOf :AmbientProperty .

:Service
      a       owl:Class ;
      rdfs:comment "A service is a set of distinct capabilities provided by a software component through a defined interface, which may be composed of other services. A service is implemented by one or more components. A service defines network interfaces and exposed by an Endpoint. (definition taken from ISO/IEC 11404:2007)"@en ;
      rdfs:label "Service"@en ;
      rdfs:seeAlso "ISO/IEC CC 30141. Information technology - Internet of Things Reference architecutre (IoT RA)"@en ;
      rdfs:subClassOf :VirtualThing .

:EVCharger
      a       owl:Class ;
      rdfs:label "Electric vehicle charging point"@en , "Electric vehicle chargeren" ;
      rdfs:subClassOf :Charger .
